testdata/cue/let_not_in_output.cue
@@ -1,0 +1,4 @@
+let secret = "abc"
+
+shown: secret
+other: 1
