testdata/cue/let_shadow.cue
@@ -1,0 +1,7 @@
+let v = 1
+
+outer: v
+inner: {
+	let v = 2
+	val: v
+}
