testdata/cue/let_sibling.cue
@@ -1,0 +1,5 @@
+top: {
+	base: 10
+	let doubled = base * 2
+	out: doubled
+}
